theories/examples/encoding_proofs.v
@@ -1,13 +1,12 @@
 From iris.proofmode Require Import tactics.
 From iris.program_logic Require Export weakestpre.
 From iris.heap_lang Require Import proofmode notation.
-From osiris Require Import typing channel logrel.
 From iris.algebra Require Import list auth excl.
 From iris.base_logic Require Import invariants.
-From osiris Require Import encodable.
-From osiris Require Import examples.
+From osiris.encodings Require Import stype_enc.
+From osiris.examples Require Import examples.
 
-Section Encodings_Examples.
+Section ExampleProofsEncodings.
   Context `{!heapG Σ} {N : namespace}.
   Context `{!logrelG val Σ}.
 
@@ -116,4 +115,4 @@ Section Encodings_Examples.
       by iApply "HΦ".
   Qed.
 
-End Encodings_Examples.
+End ExampleProofsEncodings.
