theories/examples/proofs.v
@@ -1,9 +1,10 @@
 From iris.proofmode Require Import tactics.
 From iris.program_logic Require Export weakestpre.
 From iris.heap_lang Require Import proofmode notation.
-From osiris Require Import typing channel logrel.
 From iris.base_logic Require Import invariants.
-From osiris Require Import examples.
+From osiris.typing Require Import side stype.
+From osiris.encodings Require Import stype.
+From osiris.examples Require Import examples.
 
 Section ExampleProofs.
   Context `{!heapG Σ} (N : namespace).
