theories/typing/side.v
@@ -1,0 +1,9 @@
+From iris.heap_lang Require Import proofmode notation.
+From osiris.typing Require Export involutive.
+
+Inductive side := Left | Right.
+Instance side_inhabited : Inhabited side := populate Left.
+Definition dual_side (s : side) : side :=
+  match s with Left => Right | Right => Left end.
+Instance dual_side_involutive : Involutive (=) dual_side.
+Proof. by intros []. Qed.
